Going for equivs

proof/correctness/avx2/MLKEM_avx2_equivs_mr.ec
@@ -37,6 +37,410 @@ import MLKEM_PolyvecAVX.
 import MLKEM_PolyAVXVec.
 import MLKEM_PolyVecAVXVec.
 
+
+import BitEncoding.BitChunking.
+
+require import Array128 WArray128.
+
+
+timeout 1.
+
+(*************************)
+(*************************)
+(* BEGIN BINDINGS        *)
+(*************************)
+(*************************)
+(*************************)
+
+require import QFABV.
+
+theory W4.
+  abbrev [-printing] size = 4.
+  clone include BitWordSH with op size <- size
+  rename "_XX" as "_4"
+  proof gt0_size by done,
+        size_le_256 by done.
+
+end W4. export W4 W4.ALU W4.SHIFT.
+
+bind bitstring W4.w2bits W4.bits2w W4.t 4.
+realize ge0_size by auto.
+realize size_tolist by exact W4.size_w2bits.
+realize tolistK by exact W4.w2bitsK.
+realize oflistK by exact W4.bits2wK.
+bind bitstring W256.w2bits W256.bits2w W256.t 256.
+realize ge0_size by auto.
+realize size_tolist by exact W256.size_w2bits.
+realize tolistK by exact W256.w2bitsK.
+realize oflistK by exact W256.bits2wK.
+bind bitstring W64.w2bits W64.bits2w W64.t 64.
+realize ge0_size by auto.
+realize size_tolist by exact W64.size_w2bits.
+realize tolistK by exact W64.w2bitsK.
+realize oflistK by exact W64.bits2wK.
+bind bitstring W32.w2bits W32.bits2w W32.t 32.
+realize ge0_size by auto.
+realize size_tolist by exact W32.size_w2bits.
+realize tolistK by exact W32.w2bitsK.
+realize oflistK by exact W32.bits2wK.
+bind bitstring W16.w2bits W16.bits2w W16.t 16.
+realize ge0_size by auto.
+realize size_tolist by exact W16.size_w2bits.
+realize tolistK by exact W16.w2bitsK.
+realize oflistK by exact W16.bits2wK.
+bind bitstring W8.w2bits W8.bits2w W8.t 8.
+realize ge0_size by auto.
+realize size_tolist by exact W8.size_w2bits.
+realize tolistK by exact W8.w2bitsK.
+realize oflistK by exact W8.bits2wK.
+bind circuit VPSUB_16u16 "VPSUB_16u16".
+bind circuit VPSRA_16u16 "VPSRA_16u16".
+bind circuit VPADD_16u16 "VPADD_16u16".
+bind circuit W256.(`&`) "AND_256".
+bind circuit VPBROADCAST_16u16 "VPBROADCAST_16u16".
+bind circuit VPMULH_16u16 "VPMULH_16u16".
+bind circuit VPMULHRS_16u16 "VPMULHRS_16u16".
+bind circuit VPACKUS_16u16 "VPACKUS_16u16".
+bind circuit VPMADDUBSW_256 "VPMADDUBSW_256".
+bind circuit VPERMD "VPERMD".
+
+
+bind op W16.(+) "bvadd".
+realize bvaddP. 
+move => bv1 bv2.
+by rewrite /BV_W16_t.toint -!W16.to_uintE !W16.to_uintD W16.to_uintE.
+qed.
+
+bind op W64.(+) "bvadd".
+realize bvaddP. 
+move => bv1 bv2.
+by rewrite /BV_W64_t.toint -!W64.to_uintE !W64.to_uintD W64.to_uintE.
+qed.
+
+op sliceget_256_256_16(a : W16.t Array256.t, i : int) : W256.t =
+   WArray512.get256 (WArray512.init16 (fun (i_0 : int) => a.[i_0])) i.
+
+lemma sliceget_256_256_16E (a : W16.t Array256.t) (i : int) :
+   WArray512.get256 (WArray512.init16 (fun (i_0 : int) => a.[i_0])) i = 
+    sliceget_256_256_16 a i by auto.
+
+op sliceset_256_256_16(a : W16.t Array256.t,i : int, x : W256.t) : W16.t Array256.t =
+   Array256.init (fun (i0 : int) => WArray512.get16 (WArray512.set256 ((WArray512.init16 (fun (i_0 : int) => a.[i_0]))) i x) i0).
+
+lemma sliceset_256_256_16E  (a : W16.t Array256.t) (i : int) (x  : W256.t) :
+  Array256.init (fun (i0 : int) => WArray512.get16 (WArray512.set256 ((WArray512.init16 (fun (i_0 : int) => a.[i_0]))) i x) i0) = 
+   sliceset_256_256_16 a i x by auto.
+
+op sliceget_256_16_16(a : W16.t Array16.t, i : int) : W256.t =
+   WArray32.get256 (WArray32.init16 (fun (i_0 : int) => a.[i_0])) i.
+
+lemma sliceget_256_16_16E (a : W16.t Array16.t) (i : int) :
+   WArray32.get256 (WArray32.init16 (fun (i_0 : int) => a.[i_0])) i = 
+    sliceget_256_16_16 a i by auto.
+
+op sliceget_256_8_32(a : W32.t Array8.t, i : int) : W256.t =
+   WArray32.get256 (WArray32.init32 (fun (i_0 : int) => a.[i_0])) i.
+
+lemma sliceget_256_8_32E (a : W32.t Array8.t) (i : int) :
+   WArray32.get256 (WArray32.init32 (fun (i_0 : int) => a.[i_0])) i = 
+    sliceget_256_8_32 a i by auto.
+
+op sliceset_256_128_8(a : W8.t Array128.t,i : int, x : W256.t) : W8.t Array128.t =
+   Array128.init ((WArray128.get8 ((WArray128.set256 ((WArray128.init8 (fun (i_0 : int) => a.[i_0]))) i x)))).
+
+lemma sliceset_256_128_8E  (a : W8.t Array128.t) (i : int) (x  : W256.t) :
+  Array128.init ((WArray128.get8 ((WArray128.set256 ((WArray128.init8 (fun (i_0 : int) => a.[i_0]))) i x)))) = 
+   sliceset_256_128_8 a i x by auto.
+
+
+bind bitstring circuit Array256."_.[_]" Array256."_.[_<-_]" Array256.to_list (W16.t Array256.t) 256.
+
+bind bitstring circuit Array16."_.[_]" Array16."_.[_<-_]" Array16.to_list (W16.t Array16.t) 16.
+
+bind bitstring circuit Array128."_.[_]" Array128."_.[_<-_]" Array128.to_list (W8.t Array128.t) 128.
+
+bind bitstring circuit Array8."_.[_]" Array8."_.[_<-_]" Array8.to_list (W32.t Array8.t) 8.
+
+(*************************)
+(*************************)
+(* END BINDINGS          *)
+(*************************)
+(*************************)
+(*************************)
+
+(*************************)
+(*************************)
+(* begin aux lemmas      *)
+(*************************)
+(*************************)
+(*************************)
+
+
+lemma get_vs_bits_256u16_size(wa : W16.t Array256.t) :
+   size (chunk 16 (flatten [flatten (map W16.w2bits (to_list wa))])) = 256.
+     rewrite flatten1 size_chunk // size_flatten // -map_comp /(\o). 
+     rewrite (eq_map _ (fun _ => 16)) => //=.
+     have -> : map (fun (_ : W16.t) => 16) (to_list wa) =
+               mkseq (fun _ => 16) 256; last 
+        by rewrite /mkseq -iotaredE /= /sumz /=. 
+     apply (eq_from_nth witness).
+     + by rewrite size_map Array256.size_to_list size_mkseq /#.
+     move => i.
+     rewrite size_map Array256.size_to_list => ib.
+     rewrite (nth_map witness) /=;1: by smt(Array256.size_to_list).
+     by rewrite (nth_mkseq) /#.
+qed.
+
+lemma get_vs_bits_256u16(wa : W16.t Array256.t) k :
+  0 <= k < 256 =>
+  nth witness (map W16.bits2w (chunk 16 (flatten [flatten (map W16.w2bits (to_list wa))]))) k = wa.[k].
+move => kb.
+  rewrite (nth_map witness);1:smt(get_vs_bits_256u16_size size_map).
+  rewrite  (nth_change_dfl [] witness);
+     1: by smt(get_vs_bits_256u16_size). 
+  rewrite JWordList.nth_chunk //; move : kb => [#kb0 kb1] //.
+  rewrite flatten1 size_flatten  /= /sumz /=. 
+  + have -> : (map List.size (map W16.w2bits (to_list wa))) = 
+         mkseq (fun _ => 16) 256.
+     apply (eq_from_nth witness);1:
+      by rewrite !size_map size_iota. 
+    move => i. rewrite !size_map size_iota /max /= => ib.
+    rewrite nth_mkseq 1:/# /=.
+    rewrite (nth_map witness);1:by rewrite size_map Array256.size_to_list /#.
+    rewrite (nth_map witness); 1:by rewrite  Array256.size_to_list /#.
+    by rewrite size_w2bits.
+  by rewrite /mkseq -iotaredE /= /#.
+  rewrite flatten1 drop_flatten_ctt.
+  by move => x; rewrite mapP => H;elim H => x0; smt(W16.size_w2bits).
+  rewrite -map_drop. 
+  rewrite (: 16 = 16*1) 1:/# take_flatten_ctt.
+  by move => x; rewrite mapP => H;elim H => x0; smt(W16.size_w2bits).
+  rewrite -map_take (drop_take1_nth witness) /=;1:smt(Array256.size_to_list).
+  by rewrite flatten1 w2bitsK.
+qed.
+
+lemma get_vs_bits_pre_256u16 (wa : W16.t Array256.t) (f : W16.t -> bool) (g : W16.t -> bool) :  (forall x, f x => g x) => 
+   (forall (k : int), 0 <= k && k < 256 => f wa.[k]) =>
+         all g (map W16.bits2w (chunk 16 (flatten [flatten (map W16.w2bits (to_list wa))]))).
+proof. 
+  move => H H0.
+  apply (all_nthP _ _ witness) => k kb /=.
+  by rewrite get_vs_bits_256u16;smt(get_vs_bits_256u16_size size_map).
+qed.
+
+(*************************)
+(*************************)
+(* end aux lemmas        *)
+(*************************)
+(*************************)
+(*************************)
+
+print Jkem.M.
+
+module Aux(SC : Jkem.Syscall_t) = {
+proc _poly_csubq(rp : W16.t Array256.t) : W16.t Array256.t = {
+    var i : int;
+    var t : W16.t;
+    var b : W16.t;
+    
+    i <- 0;
+    while (i < 256){
+      t <- rp.[i];
+      t <- t - (of_int 3329)%W16;
+      b <- t;
+      b <- b `|>>` (of_int 15)%W8;
+      b <- b `&` (of_int 3329)%W16;
+      t <- t + b;
+      rp.[i] <- t;
+      i <- i + 1;
+    }
+    
+    return rp;
+  }
+
+proc __polyvec_csubq(r : W16.t Array768.t) : W16.t Array768.t = {
+    var aux : W16.t Array256.t;
+    
+    aux <@ _poly_csubq((init (fun (i : int) => r.[0 + i]))%Array256);
+    r <- (init (fun (i : int) => if 0 <= i && i < 0 + 256 then aux.[i - 0] else r.[i]))%Array768;
+    aux <@ _poly_csubq((init (fun (i : int) => r.[256 + i]))%Array256);
+    r <- (init (fun (i : int) => if 256 <= i && i < 256 + 256 then aux.[i - 256] else r.[i]))%Array768;
+    aux <@ _poly_csubq((init (fun (i : int) => r.[2 * 256 + i]))%Array256);
+    r <- (init (fun (i : int) => if 2 * 256 <= i && i < 2 * 256 + 256 then aux.[i - 2 * 256] else r.[i]))%Array768;
+    
+    return r;
+  }
+  
+
+proc __i_polyvec_compress(rp : W8.t Array960.t, a : W16.t Array768.t) : W8.t Array960.t = {
+    var aux : int;
+    var i : int;
+    var j : int;
+    var aa : W16.t Array768.t;
+    var k : int;
+    var t : W64.t Array4.t;
+    var c : W16.t;
+    var b : W16.t;
+    
+    aa <- witness;
+    t <- witness;
+    i <- 0;
+    j <- 0;
+    aa <@ __polyvec_csubq(a);
+    while (i < (3 * 256 - 3)){
+      k <- 0;
+      while (k < 4){
+        t.[k] <- zeroextu64 aa.[i+k];
+        t.[k] <- t.[k] `<<` (of_int 10)%W8;
+        t.[k] <- t.[k] + (of_int 1665)%W64;
+        t.[k] <- t.[k] * (of_int 1290167)%W64;
+        t.[k] <- t.[k] `>>` (of_int 32)%W8;
+        t.[k] <- t.[k] `&` (of_int 1023)%W64;
+        k <- k + 1;
+      }
+      c <- truncateu16 t.[0];
+      c <- c `&` (of_int 255)%W16;
+      rp.[j] <- truncateu8 c;
+      j <- j + 1;
+      b <- truncateu16 t.[0];
+      b <- b `>>` (of_int 8)%W8;
+      c <- truncateu16 t.[1];
+      c <- c `<<` (of_int 2)%W8;
+      c <- c `|` b;
+      rp.[j] <- truncateu8 c;
+      j <- j + 1;
+      b <- truncateu16 t.[1];
+      b <- b `>>` (of_int 6)%W8;
+      c <- truncateu16 t.[2];
+      c <- c `<<` (of_int 4)%W8;
+      c <- c `|` b;
+      rp.[j] <- truncateu8 c;
+      j <- j + 1;
+      b <- truncateu16 t.[2];
+      b <- b `>>` (of_int 4)%W8;
+      c <- truncateu16 t.[3];
+      c <- c `<<` (of_int 6)%W8;
+      c <- c `|` b;
+      rp.[j] <- truncateu8 c;
+      j <- j + 1;
+      t.[3] <- t.[3] `>>` (of_int 2)%W8;
+      rp.[j] <- truncateu8 t.[3];
+      j <- j + 1;
+      i <- i + 4;
+    }
+    
+    return rp;
+  }
+  
+}.
+
+
+equiv auxcsubq : Jkem.M(Jkem.Syscall)._poly_csubq ~ Aux(Jkem.Syscall)._poly_csubq : ={arg} ==> ={res}.
+proc. 
+while(={rp} /\ to_uint i{1} = i{2} /\ 0 <= i{2} <= 256).
++ auto => /> &1;rewrite !ultE /= => ????.
+  rewrite !to_uintD_small /=; smt().
+by auto.
+qed.
+
+equiv auxcsubqv : Jkem.M(Jkem.Syscall).__polyvec_csubq ~ Aux(Jkem.Syscall).__polyvec_csubq : ={arg} ==> ={res}.
+proc.
+do 3!(wp;call auxcsubq).
+by auto => />.
+qed.
+
+equiv auxcompress : Jkem.M(Jkem.Syscall).__i_polyvec_compress ~ Aux(Jkem.Syscall).__i_polyvec_compress : ={arg} ==> ={res}.
+proc.
+while (0<=i{2}<=768 /\ to_uint i{1} = i{2} /\ to_uint j{1} = j{2} /\ to_uint j{1} * 4 = i{2} * 5 /\ ={rp,aa}).
++ unroll for {1} 2; unroll for {2} 2; auto => /> &1. 
+  by rewrite !ultE /= => &2????;rewrite !to_uintD_small /=; smt().
+by call auxcsubqv;auto => />.
+qed.
+
+equiv compressequivvec_1 mem : 
+ Jkem_avx2.M(Jkem_avx2.Syscall).__polyvec_compress_1 ~  Jkem.M(Jkem.Syscall).__i_polyvec_compress :
+     pos_bound768_cxq a{1} 0 768 2 /\
+     pos_bound768_cxq a{2} 0 768 2 /\
+    lift_array768 a{1} = lift_array768 a{2} /\ 
+    ={Glob.mem} /\ Glob.mem{1} = mem 
+    ==> 
+    ={Glob.mem,res} /\  Glob.mem{1} = mem.
+proof.
+proc. 
+  transitivity MLKEM_PolyVec_avx2_prevec.Mprevec.polyvec_compress_1
+               (={rp, a, Glob.mem} ==> ={res, Glob.mem})
+               (pos_bound768_cxq a{1} 0 768 2 /\
+                pos_bound768_cxq a{2} 0 768 2 /\
+                lift_array768 a{1} = lift_array768 a{2} /\ ={Glob.mem} /\ Glob.mem{1} = mem
+                 ==>
+                ={Glob.mem, res} /\ Glob.mem{2} = mem); 1,2: smt().
+    + symmetry. proc * => /=. call prevec_eq_polyvec_compress_1 => //=.
+  transitivity EncDec_AVX2.encode10_opt_vec
+               (a{2} = compress_polyvec 10  (lift_polyvec a{1}) /\
+                pos_bound768_cxq a{1} 0 768 2 /\ (forall i, 0<=i<768 => 0 <= a{2}.[i] < q) /\
+                Glob.mem{1} = mem /\ ={Glob.mem} ==>
+                Glob.mem{1} = mem /\
+                ={res})
+               (pos_bound768_cxq a{2} 0 768 2 /\ (forall i, 0<=i<768 => 0 <= a{1}.[i] < q) /\
+                a{1} = compress_polyvec 10 (lift_polyvec a{2}) /\
+                Glob.mem{2} = mem /\ ={Glob.mem} ==>
+                Glob.mem{2} = mem /\
+                ={res}).
+    auto => &1 &2 [#] pos_bound_al pos_bound_ar al_eq_ar />.
+    exists Glob.mem{2}.
+      exists (compress_polyvec 10 (lift_polyvec a{1})).
+        rewrite pos_bound_al pos_bound_ar /=.
+        do split.
+        + move => i ib; rewrite /compress_polyvec /lift_polyvec !mapiE //=.
+          pose x := fromarray256 _ _ _.
+          move : (compress_rng x.[i] 10 _) => //=; smt (qE).
+        + move => i ib; rewrite /compress_polyvec /lift_polyvec !mapiE //=.
+          pose x := fromarray256 _ _ _.
+          move : (compress_rng x.[i] 10 _) => //=; smt (qE).
+        + congr; rewrite /lift_polyvec KMatrix.Vector.eq_vectorP => i ib /=.
+          rewrite !KMatrix.Vector.offunvE /kvec //=.
+          rewrite /lift_array768 /subarray256 /lift_array256 tP => k kb.
+          rewrite !mapiE //= !initiE //=.
+          smt(@Array768).
+        + smt().
+    + proc * => /=.
+      ecall (polyvec_compress_1_corr (lift_polyvec a{1})  mem) => //=.
+  symmetry.
+  transitivity EncDec.encode10_vec
+               (u{2} = compress_polyvec 10 (lift_polyvec a{1}) /\
+                pos_bound768_cxq a{1} 0 768 2 /\ (forall i, 0<=i<768 => 0 <= u{2}.[i] < q) /\
+                Glob.mem{1} = mem /\ ={Glob.mem} ==>
+                Glob.mem{1} = mem /\ ={res})
+               ((forall i, 0<=i<768 => 0 <= u{1}.[i] < q) /\
+                u{1} = a{2} /\
+                ={Glob.mem} ==> ={Glob.mem, res}).
+               auto => &1 &2 [#] pos_bound_a a2_bnd a1_eq_a2 mem_eq />.
+               exists Glob.mem{1}.
+                 exists (compress_polyvec 10 (lift_polyvec a{1})).
+                   auto => />;do split.
+                   + move => i ibl ibh; rewrite /compress_polyvec /lift_polyvec !mapiE //=.
+                     pose x := fromarray256 _ _ _.
+                     move : (compress_rng x.[i] 10 _) => //=; smt (qE).
+                   + move => i ibl ibh; rewrite /compress_polyvec /lift_polyvec !mapiE //=.
+                     pose x := fromarray256 _ _ _.
+                     move : (compress_rng x.[i] 10 _) => //=; smt (qE).
+                   + smt().
+               smt().
+    + proc * => /=.
+      ecall (MLKEM_PolyVec.i_polyvec_compress_corr (lift_array768 a{1})) => //=.
+      auto => /> &1 H H0.
+        + rewrite /compress_polyvec; congr.
+          rewrite /fromarray256 /lift_polyvec /lift_array768 tP => i ib /=.
+          rewrite !initiE //= !mapiE //= !getvE !KMatrix.Vector.offunvE //=.
+          rewrite /subarray256 /lift_array256 /=.
+          smt(@Array256).
+  symmetry.
+  proc * => /=.
+  call encode10_opt_corr.
+  auto => />.
+qed.
+
+
 lemma polyvec_decompress_equiv mem _p :
     equiv [Jkem_avx2.M(Jkem_avx2.Syscall).__polyvec_decompress ~  Jkem.M(Jkem.Syscall).__polyvec_decompress  :
              valid_ptr _p (3*320) /\
@@ -240,87 +644,6 @@ proof.
   auto => />.
 qed.
 
-equiv compressequivvec_1 mem : 
- Jkem_avx2.M(Jkem_avx2.Syscall).__polyvec_compress_1 ~  Jkem.M(Jkem.Syscall).__i_polyvec_compress :
-     pos_bound768_cxq a{1} 0 768 2 /\
-     pos_bound768_cxq a{2} 0 768 2 /\
-    lift_array768 a{1} = lift_array768 a{2} /\ 
-    ={Glob.mem} /\ Glob.mem{1} = mem 
-    ==> 
-    ={Glob.mem,res} /\  Glob.mem{1} = mem.
-proof.
-  transitivity MLKEM_PolyVec_avx2_prevec.Mprevec.polyvec_compress_1
-               (={rp, a, Glob.mem} ==> ={res, Glob.mem})
-               (pos_bound768_cxq a{1} 0 768 2 /\
-                pos_bound768_cxq a{2} 0 768 2 /\
-                lift_array768 a{1} = lift_array768 a{2} /\ ={Glob.mem} /\ Glob.mem{1} = mem
-                 ==>
-                ={Glob.mem, res} /\ Glob.mem{2} = mem); 1,2: smt().
-    + symmetry. proc * => /=. call prevec_eq_polyvec_compress_1 => //=.
-  transitivity EncDec_AVX2.encode10_opt_vec
-               (a{2} = compress_polyvec 10  (lift_polyvec a{1}) /\
-                pos_bound768_cxq a{1} 0 768 2 /\ (forall i, 0<=i<768 => 0 <= a{2}.[i] < q) /\
-                Glob.mem{1} = mem /\ ={Glob.mem} ==>
-                Glob.mem{1} = mem /\
-                ={res})
-               (pos_bound768_cxq a{2} 0 768 2 /\ (forall i, 0<=i<768 => 0 <= a{1}.[i] < q) /\
-                a{1} = compress_polyvec 10 (lift_polyvec a{2}) /\
-                Glob.mem{2} = mem /\ ={Glob.mem} ==>
-                Glob.mem{2} = mem /\
-                ={res}).
-    auto => &1 &2 [#] pos_bound_al pos_bound_ar al_eq_ar />.
-    exists Glob.mem{2}.
-      exists (compress_polyvec 10 (lift_polyvec a{1})).
-        rewrite pos_bound_al pos_bound_ar /=.
-        do split.
-        + move => i ib; rewrite /compress_polyvec /lift_polyvec !mapiE //=.
-          pose x := fromarray256 _ _ _.
-          move : (compress_rng x.[i] 10 _) => //=; smt (qE).
-        + move => i ib; rewrite /compress_polyvec /lift_polyvec !mapiE //=.
-          pose x := fromarray256 _ _ _.
-          move : (compress_rng x.[i] 10 _) => //=; smt (qE).
-        + congr; rewrite /lift_polyvec KMatrix.Vector.eq_vectorP => i ib /=.
-          rewrite !KMatrix.Vector.offunvE /kvec //=.
-          rewrite /lift_array768 /subarray256 /lift_array256 tP => k kb.
-          rewrite !mapiE //= !initiE //=.
-          smt(@Array768).
-        + smt().
-    + proc * => /=.
-      ecall (polyvec_compress_1_corr (lift_polyvec a{1})  mem) => //=.
-  symmetry.
-  transitivity EncDec.encode10_vec
-               (u{2} = compress_polyvec 10 (lift_polyvec a{1}) /\
-                pos_bound768_cxq a{1} 0 768 2 /\ (forall i, 0<=i<768 => 0 <= u{2}.[i] < q) /\
-                Glob.mem{1} = mem /\ ={Glob.mem} ==>
-                Glob.mem{1} = mem /\ ={res})
-               ((forall i, 0<=i<768 => 0 <= u{1}.[i] < q) /\
-                u{1} = a{2} /\
-                ={Glob.mem} ==> ={Glob.mem, res}).
-               auto => &1 &2 [#] pos_bound_a a2_bnd a1_eq_a2 mem_eq />.
-               exists Glob.mem{1}.
-                 exists (compress_polyvec 10 (lift_polyvec a{1})).
-                   auto => />;do split.
-                   + move => i ibl ibh; rewrite /compress_polyvec /lift_polyvec !mapiE //=.
-                     pose x := fromarray256 _ _ _.
-                     move : (compress_rng x.[i] 10 _) => //=; smt (qE).
-                   + move => i ibl ibh; rewrite /compress_polyvec /lift_polyvec !mapiE //=.
-                     pose x := fromarray256 _ _ _.
-                     move : (compress_rng x.[i] 10 _) => //=; smt (qE).
-                   + smt().
-               smt().
-    + proc * => /=.
-      ecall (MLKEM_PolyVec.i_polyvec_compress_corr (lift_array768 a{1})) => //=.
-      auto => /> &1 H H0.
-        + rewrite /compress_polyvec; congr.
-          rewrite /fromarray256 /lift_polyvec /lift_array768 tP => i ib /=.
-          rewrite !initiE //= !mapiE //= !getvE !KMatrix.Vector.offunvE //=.
-          rewrite /subarray256 /lift_array256 /=.
-          smt(@Array256).
-  symmetry.
-  proc * => /=.
-  call encode10_opt_corr.
-  auto => />.
-qed.
 
 lemma poly_decompress_equiv mem _p : 
     equiv [Jkem_avx2.M(Jkem_avx2.Syscall)._poly_decompress ~  Jkem.M(Jkem.Syscall)._poly_decompress  :
