proof/correctness/avx2/MLKEM_Poly_avx2_proof_mr.ec
@@ -25,12 +25,6 @@ import BitEncoding.BitChunking.
 
 timeout 1.
 
-require import AllCore List.
-from Jasmin require import JModel.
-import BitEncoding.BitChunking.
-
-require import MLKEMFCLib.
-require import Array8 Array256 WArray512 Array16 WArray32 Array128 WArray128.
 (*************************)
 (*************************)
 (* BEGIN BINDINGS        *)
